start on provability

language_term_n2.lean
@@ -4,10 +4,11 @@ meta def congr1 : tactic unit := congr_core
 end interactive
 end tactic
 
+namespace fol
 structure Language := 
-(relations : Π n : nat, Type) (functions : Π  n : nat, Type)
+(relations : ℕ → Type) (functions : ℕ → Type) (equal : relations 2) (false : relations 0)
 section
-parameter L : Language
+parameter {L : Language}
 
 /- preterm n is a partially applied term. if applied to n terms, it becomes a term -/
 inductive preterm : ℕ → Type 
@@ -15,41 +16,46 @@ inductive preterm : ℕ → Type
 | func : ∀ {n : nat}, L.functions n → preterm n
 | apply : ∀ {n : nat}, preterm (n + 1) → preterm 0 → preterm n
 open preterm
-def term := preterm 0
+@[reducible] def term := preterm 0
 
-/- lift_term _ t n m raises variables in t which are at least m by n -/
-@[simp] def lift_term : ∀ {l}, preterm l → ℕ → ℕ → preterm l
-| _ (var L k)     n m := if m ≤ k then var (k+n) else var k
+local prefix `&`:max := var
+
+/- lift_term_at _ t n m raises variables in t which are at least m by n -/
+@[simp] def lift_term_at : ∀ {l}, preterm l → ℕ → ℕ → preterm l
+| _ (var k)       n m := if m ≤ k then var (k+n) else var k
 | _ (func f)      n m := func f
-| _ (apply t1 t2) n m := apply (lift_term t1 n m) (lift_term t2 n m)
+| _ (apply t1 t2) n m := apply (lift_term_at t1 n m) (lift_term_at t2 n m)
 
-local notation [parsing_only] t ` ↑ `:55 n ` # `:55 m:55 := lift_term t n m
+local notation t ` ↑ `:55 n ` # `:55 m:55 := lift_term_at t n m
 
-lemma lift_term_inj : ∀ {l} {t t' : preterm l} {n m : ℕ}, t ↑ n # m = t' ↑ n # m → t = t'
-| _ (var L k) (var .(L) k')   n m h := 
+def lift_term (t : term) (n : ℕ) : term := t ↑ n # 0
+def lift_term1 (t : term) : term := t ↑ 1 # 0
+
+lemma lift_term_at_inj : ∀ {l} {t t' : preterm l} {n m : ℕ}, t ↑ n # m = t' ↑ n # m → t = t'
+| _ (var k) (var k')          n m h := 
   by by_cases h₁ : m ≤ k; by_cases h₂ : m ≤ k'; simp [h₁, h₂] at h; congr; 
        [exact add_right_cancel h, skip, skip, assumption]; exfalso; 
        try {apply h₁}; try {apply h₂}; subst h; 
        apply le_trans (by assumption) (nat.le_add_right _ _)
-| _ (var L k) (func f')       n m h := by by_cases h' : m ≤ k; simp [h'] at h; contradiction
-| _ (var L k) (apply t1' t2') n m h := by by_cases h' : m ≤ k; simp [h'] at h; contradiction
-| _ (func f) (var .(L) k')    n m h := by by_cases h' : m ≤ k'; simp [h'] at h; contradiction
+| _ (var k) (func f')         n m h := by by_cases h' : m ≤ k; simp [h'] at h; contradiction
+| _ (var k) (apply t1' t2')   n m h := by by_cases h' : m ≤ k; simp [h'] at h; contradiction
+| _ (func f) (var k')         n m h := by by_cases h' : m ≤ k'; simp [h'] at h; contradiction
 | _ (func f) (func f')        n m h := h
 | _ (func f) (apply t1' t2')  n m h := by cases h
-| _ (apply t1 t2) (var _ k')  n m h := by by_cases h' : m ≤ k'; simp [h'] at h; contradiction
+| _ (apply t1 t2) (var k')    n m h := by by_cases h' : m ≤ k'; simp [h'] at h; contradiction
 | _ (apply t1 t2) (func f')   n m h := by cases h
 | _ (apply t1 t2) (apply t1' t2') n m h := 
-  begin injection h, congr; apply lift_term_inj; assumption end
+  begin injection h, congr; apply lift_term_at_inj; assumption end
 
-@[simp] lemma lift_term_zero : ∀ {l} (t : preterm l) (m : ℕ), t ↑ 0 # m = t
-| _ (var L k)     m := by simp
+@[simp] lemma lift_term_at_zero : ∀ {l} (t : preterm l) (m : ℕ), t ↑ 0 # m = t
+| _ (var k)     m := by simp
 | _ (func f)      m := by refl
-| _ (apply t1 t2) m := by dsimp; congr; apply lift_term_zero
+| _ (apply t1 t2) m := by dsimp; congr; apply lift_term_at_zero
 
 /- the following lemmas simplify iterated lifts, depending on the size of m' -/
-lemma lift_term2_small : ∀ {l} (t : preterm l) (n n') {m m'}, m' ≤ m → 
+lemma lift_term_at2_small : ∀ {l} (t : preterm l) (n n') {m m'}, m' ≤ m → 
   (t ↑ n # m) ↑ n' # m' = (t ↑ n' # m') ↑ n # (m + n')
-| _ (var L k)     n n' m m' H := 
+| _ (var k)       n n' m m' H := 
   begin 
     by_cases h : m ≤ k,
     { have h₁ : m' ≤ k, from le_trans H h,
@@ -62,11 +68,11 @@ lemma lift_term2_small : ∀ {l} (t : preterm l) (n n') {m m'}, m' ≤ m →
   end
 | _ (func f)      n n' m m' H := by refl
 | _ (apply t1 t2) n n' m m' H := 
-  begin dsimp; congr1; apply lift_term2_small; assumption end
+  begin dsimp; congr1; apply lift_term_at2_small; assumption end
 
-lemma lift_term2_medium : ∀ {l} (t : preterm l) (n n') {m m'}, m ≤ m' → m' ≤ m+n → 
+lemma lift_term_at2_medium : ∀ {l} (t : preterm l) (n n') {m m'}, m ≤ m' → m' ≤ m+n → 
   (t ↑ n # m) ↑ n' # m' = t ↑ (n+n') # m
-| _ (var L k)     n n' m m' H₁ H₂ := 
+| _ (var k)       n n' m m' H₁ H₂ := 
   begin 
     by_cases h : m ≤ k,
     { have h₁ : m' ≤ k + n, from le_trans H₂ (add_le_add_right h n),
@@ -77,28 +83,36 @@ lemma lift_term2_medium : ∀ {l} (t : preterm l) (n n') {m m'}, m ≤ m' → m'
   end
 | _ (func f)      n n' m m' H₁ H₂ := by refl
 | _ (apply t1 t2) n n' m m' H₁ H₂ := 
-  begin dsimp; congr1; apply lift_term2_medium; assumption end
+  begin dsimp; congr1; apply lift_term_at2_medium; assumption end
 
-lemma lift_term2_eq {l} (t : preterm l) (n n' m : ℕ) : 
+lemma lift_term_at2_eq {l} (t : preterm l) (n n' m : ℕ) : 
   (t ↑ n # m) ↑ n' # (m+n) = t ↑ (n+n') # m :=
-lift_term2_medium t n n' (m.le_add_right n) (le_refl _)
+lift_term_at2_medium t n n' (m.le_add_right n) (le_refl _)
 
-lemma lift_term2_large {l} (t : preterm l) (n n') {m m'} (H : m' ≥ m + n) : 
+lemma lift_term_at2_large {l} (t : preterm l) (n n') {m m'} (H : m' ≥ m + n) : 
   (t ↑ n # m) ↑ n' # m' = (t ↑ n' # m'-n) ↑ n # m :=
 have H₁ : n ≤ m', from le_trans (n.le_add_left m) H,
 have H₂ : m ≤ m' - n, by rw [←nat.add_sub_cancel m n]; apply nat.sub_le_sub_right; exact H,
-begin rw lift_term2_small t n' n H₂, rw [nat.sub_add_cancel], exact H₁ end
+begin rw fol.lift_term_at2_small t n' n H₂, rw [nat.sub_add_cancel], exact H₁ end
 
 /- substitute_term t s n substitutes s for (var n) and reduces the level of all variables above n by 1 -/
 @[simp] def substitute_term : ∀ {l}, preterm l → term → ℕ → preterm l
-| _ (var L k)     s n := if k < n then var k else if k > n then var (k-1) else s
+| _ (var k)     s n := if k < n then var k else if n < k then var (k-1) else s
 | _ (func f)      s n := func f
 | _ (apply t1 t2) s n := apply (substitute_term t1 s n) (substitute_term t2 s n)
 
+@[simp] def substitute_term_var_eq (t : term) (n : ℕ) : substitute_term &n t n = t :=
+by simp [lt_irrefl]
+
+lemma substitute_term_lift_term' : ∀{l} (t : preterm l) (s : term), 
+  substitute_term (lift_term_at t 1 0) s 0 = t :=
+sorry
+
+@[simp] lemma substitute_term_lift_term (t s : term) : substitute_term (lift_term1 t) s 0 = t :=
+substitute_term_lift_term' t s
+
 /- preformula n is a partially applied formula. if applied to n terms, it becomes a formula -/
 inductive preformula : ℕ → Type 
-| false : preformula 0
-| equal : term → term → preformula 0
 | rel : ∀ {n : nat}, L.relations n → preformula n
 | apprel : ∀ {n : nat}, preformula (n + 1) → term → preformula n
 | imp : preformula 0 → preformula 0 → preformula 0
@@ -106,65 +120,117 @@ inductive preformula : ℕ → Type
 open preformula
 def formula := preformula 0
 
-@[simp] def lift_formula : ∀ {l}, preformula l → ℕ → ℕ → preformula l
-| _ (false L)     n m := false
-| _ (equal t1 t2) n m := equal (lift_term t1 n m) (lift_term t2 n m)
-| _ (rel R)       n m := rel R
-| _ (apprel f t)  n m := apprel (lift_formula f n m) (lift_term t n m)
-| _ (imp f1 f2)   n m := imp (lift_formula f1 n m) (lift_formula f2 n m)
-| _ (all f)       n m := all (lift_formula f n (m+1))
+def equal (t₁ t₂ : term) : formula := apprel (apprel (rel L.equal) t₁) t₂
+def false : formula := rel L.false
+def not (f : formula) : formula := imp f false
+def or (f₁ f₂ : formula) : formula := imp (not f₁) f₂
+def and (f₁ f₂ : formula) : formula := not (imp f₁ (not f₂))
+def iff (f₁ f₂ : formula) : formula := and (imp f₁ f₂) (imp f₂ f₁)
+def ex (f : formula) : formula := not (all (not f))
 
-local notation [parsing_only] f ` ↑ `:55 n ` # `:55 m:55 := lift_formula f n m
+local infix ` ⟾ `:70 := imp
+local infix ` ⇔ `:75 := iff
+local infix ` ≍ `:80 := equal
 
-@[simp] lemma lift_formula_zero : ∀ {l} (f : preformula l) (m : ℕ), f ↑ 0 # m = f
-| _ (false L)     m := by refl
-| _ (equal t1 t2) m := by simp
-| _ (rel R)       m := by refl
-| _ (apprel f t)  m := by simp; apply lift_formula_zero
-| _ (imp f1 f2)   m := by dsimp; congr1; apply lift_formula_zero
-| _ (all f)       m := by simp; apply lift_formula_zero
+@[simp] def lift_formula_at : ∀ {l}, preformula l → ℕ → ℕ → preformula l
+| _ (rel R)      n m := rel R
+| _ (apprel f t) n m := apprel (lift_formula_at f n m) (lift_term_at t n m)
+| _ (imp f1 f2)  n m := imp (lift_formula_at f1 n m) (lift_formula_at f2 n m)
+| _ (all f)      n m := all (lift_formula_at f n (m+1))
+
+local notation f ` ↑ `:55 n ` # `:55 m:55 := lift_formula_at f n m
+
+def lift_formula (f : formula) (n : ℕ) : formula := f ↑ n # 0
+def lift_formula1 (f : formula) : formula := f ↑ 1 # 0
+
+lemma lift_formula_at_inj {l} {f f' : preformula l} {n m : ℕ} (H : f ↑ n # m = f' ↑ n # m) : f = f' :=
+begin
+  induction f generalizing m; cases f'; injection H,
+  simp [f_ih h_1, fol.lift_term_at_inj h_2],
+  simp [f_ih_a h_1, f_ih_a_1 h_2],
+  simp [f_ih h_1]
+end
+
+@[simp] lemma lift_formula_at_zero : ∀ {l} (f : preformula l) (m : ℕ), f ↑ 0 # m = f
+| _ (rel R)      m := by refl
+| _ (apprel f t) m := by simp; apply lift_formula_at_zero
+| _ (imp f1 f2)  m := by dsimp; congr1; apply lift_formula_at_zero
+| _ (all f)      m := by simp; apply lift_formula_at_zero
 
 /- the following lemmas simplify iterated lifts, depending on the size of m' -/
-lemma lift_formula2_small : ∀ {l} (f : preformula l) (n n') {m m'}, m' ≤ m → 
+lemma lift_formula_at2_small : ∀ {l} (f : preformula l) (n n') {m m'}, m' ≤ m → 
   (f ↑ n # m) ↑ n' # m' = (f ↑ n' # m') ↑ n # (m + n')
-| _ (false L)     n n' m m' H := by refl
-| _ (equal t1 t2) n n' m m' H := by simp [lift_term2_small, H]
-| _ (rel R)       n n' m m' H := by refl
-| _ (apprel f t)  n n' m m' H := 
-  by simp [lift_term2_small, H, -add_comm]; apply lift_formula2_small; assumption
-| _ (imp f1 f2)   n n' m m' H := by dsimp; congr1; apply lift_formula2_small; assumption
-| _ (all f)       n n' m m' H :=
-  by simp [lift_term2_small, H, lift_formula2_small f n n' (add_le_add_right H 1)]
+| _ (rel R)      n n' m m' H := by refl
+| _ (apprel f t) n n' m m' H := 
+  by simp [lift_term_at2_small, H, -add_comm]; apply lift_formula_at2_small; assumption
+| _ (imp f1 f2)  n n' m m' H := by dsimp; congr1; apply lift_formula_at2_small; assumption
+| _ (all f)      n n' m m' H :=
+  by simp [lift_term_at2_small, H, lift_formula_at2_small f n n' (add_le_add_right H 1)]
 
-lemma lift_formula2_medium : ∀ {l} (f : preformula l) (n n') {m m'}, m ≤ m' → m' ≤ m+n → 
+lemma lift_formula_at2_medium : ∀ {l} (f : preformula l) (n n') {m m'}, m ≤ m' → m' ≤ m+n → 
   (f ↑ n # m) ↑ n' # m' = f ↑ (n+n') # m
-| _ (false L)     n n' m m' H₁ H₂ := by refl
-| _ (equal t1 t2) n n' m m' H₁ H₂ := by simp [lift_term2_medium, H₁, H₂]
-| _ (rel R)       n n' m m' H₁ H₂ := by refl
-| _ (apprel f t)  n n' m m' H₁ H₂ :=
-  by simp [lift_term2_medium, H₁, H₂, -add_comm]; apply lift_formula2_medium; assumption
-| _ (imp f1 f2)   n n' m m' H₁ H₂ := by dsimp; congr1; apply lift_formula2_medium; assumption
-| _ (all f)       n n' m m' H₁ H₂ :=
+| _ (rel R)      n n' m m' H₁ H₂ := by refl
+| _ (apprel f t) n n' m m' H₁ H₂ :=
+  by simp [lift_term_at2_medium, H₁, H₂, -add_comm]; apply lift_formula_at2_medium; assumption
+| _ (imp f1 f2)  n n' m m' H₁ H₂ := by dsimp; congr1; apply lift_formula_at2_medium; assumption
+| _ (all f)      n n' m m' H₁ H₂ :=
   have m' + 1 ≤ (m + 1) + n, from le_trans (add_le_add_right H₂ 1) (by simp),
-  by simp [lift_term2_medium, H₁, H₂, lift_formula2_medium f n n' (add_le_add_right H₁ 1) this]
+  by simp [lift_term_at2_medium, H₁, H₂, lift_formula_at2_medium f n n' (add_le_add_right H₁ 1) this]
 
-lemma lift_formula2_eq {l} (f : preformula l) (n n' m : ℕ) : 
+lemma lift_formula_at2_eq {l} (f : preformula l) (n n' m : ℕ) : 
   (f ↑ n # m) ↑ n' # (m+n) = f ↑ (n+n') # m :=
-lift_formula2_medium f n n' (m.le_add_right n) (le_refl _)
+lift_formula_at2_medium f n n' (m.le_add_right n) (le_refl _)
 
-lemma lift_formula2_large {l} (f : preformula l) (n n') {m m'} (H : m' ≥ m + n) : 
+lemma lift_formula_at2_large {l} (f : preformula l) (n n') {m m'} (H : m' ≥ m + n) : 
   (f ↑ n # m) ↑ n' # m' = (f ↑ n' # m'-n) ↑ n # m :=
 have H₁ : n ≤ m', from le_trans (n.le_add_left m) H,
 have H₂ : m ≤ m' - n, by rw [←nat.add_sub_cancel m n]; apply nat.sub_le_sub_right; exact H,
-begin rw lift_formula2_small f n' n H₂, rw [nat.sub_add_cancel], exact H₁ end
+begin rw fol.lift_formula_at2_small f n' n H₂, rw [nat.sub_add_cancel], exact H₁ end
 
 @[simp] def substitute_formula : ∀ {l}, preformula l → term → ℕ → preformula l
-| _ (false L)     s n := false
-| _ (equal t1 t2) s n := equal (substitute_term t1 s n) (substitute_term t2 s n)
-| _ (rel R)       s n := rel R
-| _ (apprel f t)  s n := apprel (substitute_formula f s n) (substitute_term t s n)
-| _ (imp f1 f2)   s n := imp (substitute_formula f1 s n) (substitute_formula f2 s n)
-| _ (all f)       s n := all (substitute_formula f s (n+1))
+| _ (rel R)      s n := rel R
+| _ (apprel f t) s n := apprel (substitute_formula f s n) (substitute_term t s n)
+| _ (imp f1 f2)  s n := imp (substitute_formula f1 s n) (substitute_formula f2 s n)
+| _ (all f)      s n := all (substitute_formula f s (n+1))
 
+@[simp] def substitute_formula0 (f : formula) (t : term) := substitute_formula f t 0
+
+@[simp] def substitute_formula_equal (t₁ t₂ s : term) (n : ℕ) :
+  substitute_formula (t₁ ≍ t₂) s n = substitute_term t₁ s n ≍ substitute_term t₂ s n :=
+by refl
+
+-- ⟾⇔≍
+
+inductive prf : list formula → formula → Type
+| axm    : ∀{Γ A}, A ∈ Γ → prf Γ A
+| impI   : ∀{Γ A B}, prf (A::Γ) B → prf Γ (A ⟾ B)
+| impE   : ∀{Γ A B}, prf Γ (A ⟾ B) → prf Γ A → prf Γ B
+| falseE : ∀{Γ A}, prf (not A::Γ) false → prf Γ A
+| allI   : ∀{Γ A}, prf (list.map lift_formula1 Γ) A → prf Γ (all A)
+| allE   : ∀{Γ} A t, prf Γ (all A) → prf Γ (substitute_formula0 A t)
+| refl   : ∀Γ t, prf Γ (t ≍ t)
+| subst : ∀{Γ} s t f, prf Γ (s ≍ t) → prf Γ (substitute_formula f s 0) → 
+  prf Γ (substitute_formula f t 0)
+open prf
+local infix ` ⊢ `:51 := prf
+
+def symm {Γ s t} (H : Γ ⊢ s ≍ t) : Γ ⊢ t ≍ s :=
+begin 
+  have H₁ := subst s t (equal (var 0) (lift_term1 s)) H, -- why does notation not work here?
+  rw [substitute_formula_equal, substitute_formula_equal, substitute_term_lift_term, substitute_term_lift_term, substitute_term_var_eq, substitute_term_var_eq] at H₁,
+  exact H₁ (refl Γ s)
+end
+
+def trans {Γ t₁ t₂ t₃} (H : Γ ⊢ t₁ ≍ t₂) (H' : Γ ⊢ t₂ ≍ t₃) : Γ ⊢ t₁ ≍ t₃ :=
+begin 
+  have H₁ := prf.subst t₂ t₃ (equal (lift_term1 t₁) (var 0)) H', 
+  rw [substitute_formula_equal, substitute_formula_equal, substitute_term_lift_term, substitute_term_lift_term, substitute_term_var_eq, substitute_term_var_eq] at H₁,
+  exact H₁ H
+end
 
 end
+end fol
+open fol fol.preterm
+variable {L : Language}
+#check substitute_formula0 (@equal L (var 0) (var 0)) (var 7)
+#reduce substitute_formula0 (@equal L (var 0) (var 0)) (var 7)
